

ECON 6018

TUTORIAL 3

- By: Teresa Ng
- Lesson Tutorial
Date: 06/02/26

Differentiation

- the most important thing is your foundation and speed for comparative statics
- For a function to be differentiable, it has to be continuous
- welcome to my favorite Topic!

Chapt 6

Chapt 7

Chapt 11

Chapt 12

1. Derivatives and how we derive them using limits

Derivative — rate of change

- how much y change when x changes
- formula:

$$\frac{dy}{dx} = \lim_{\Delta x \rightarrow 0} \frac{\Delta y}{\Delta x} = \lim_{\Delta x \rightarrow 0} \frac{f(x_0 + \Delta x) - f(x_0)}{\Delta x}$$

- Application
maximization of utility

Questions:

Q1. Let $f(x) = 4x^2$. Show that $f(5+h) - f(5) = 40h + 4h^2$, implying that $\frac{f(5+h) - f(5)}{h} = 40 + 4h$ for $h \neq 0$. Use this result to find $f'(5)$. Compare the answer with (6.2.6).

Q2. Let $f(x) = 3x^2 + 2x - 1$.

Show that $\frac{f(x+h) - f(x)}{h} = 6x + 2 + 3h$ for $h \neq 0$, and use this result to find $f'(x)$.

Answers:

$$Q1. f(x) = 4x^2$$

$$f(5+h) - f(5) = 40h + 4h^2 \text{ (shown)}$$

$$\lim_{h \rightarrow 0} \frac{40h + 4h^2}{h} = 40$$

$$f'(5) = 40$$

$$Q2. f(x+h) = 3x^3 + 6xh + 3h^2 + 2x + 2h - 1$$

$$\frac{f(x+h) - f(x)}{h} = 6x + 3h + 2$$

$$h \rightarrow 0$$

$$f'(x) = 6x + 2$$

2. Differentiation

2.1 Basic Differentiation — chpt 6.6

Given any constant a ,

$$f(x) = x^a \Rightarrow f'(x) = ax^{a-1}$$

Questions

1. Compute the derivatives of the following functions:

(a) $y = 5$

(b) $y = x^4$

(c) $y = 9x^{10}$

(d) $y = \pi^7$

2. Suppose we know $g'(x)$. Find expressions for the derivatives of the following:

(a) $2g(x) + 3$

(b) $-\frac{1}{6}g(x) + 8$

(c) $\frac{g(x) - 5}{3}$

3. Find the derivatives of the following:

(a) x^6

(b) $3x^{11}$

(c) x^{50}

(d) $-4x^{-7}$

(e) $\frac{x^{12}}{12}$

(f) $\frac{-2}{x^2}$

(g) $\frac{3}{\sqrt[3]{x}}$

(h) $\frac{-2}{x\sqrt{x}}$

$$1(a) 0$$

$$(b) 4x^3$$

$$(c) 90x^9$$

$$(d) 0$$

$$2(a) 2g'(x)$$

$$(b) -\frac{1}{6}g'(x)$$

$$(c) \frac{g'(x)}{3}$$

$$3(a) 6x^5$$

$$(b) 33x^{10}$$

$$(c) 50x^{49}$$

$$(d) 28x^{-8}$$

$$(e) x^{11}$$

$$(f) -4x^{-3}$$

$$(g) -x^{-4/3}$$

$$(h) 3x^{-5/2}$$

2.2 Sum, Product, Quotient — chpt 6.7

a. Sum

$$F(x) = f(x) \pm g(x) \Rightarrow F'(x) = f'(x) \pm g'(x)$$

b. Product

$$F(x) = f(x) \cdot g(x) \Rightarrow F'(x) = f'(x) \cdot g(x) + f(x) \cdot g'(x)$$

c. Quotient

$$F(x) = \frac{f(x)}{g(x)} \Rightarrow F'(x) = \frac{f'(x) \cdot g(x) - f(x) \cdot g'(x)}{(g(x))^2}$$

Questions:

Q1. Differentiate w.r.t x the following functions:

(a) $x + 1$

(b) $x + x^2$

(c) $3x^5 + 2x^4 + 5$

(d) $8x^4 + 2\sqrt{x}$

(e) $\frac{1}{2}x - \frac{3}{2}x^2 + 5x^3$

(f) $1 - 3x^7$

Q2. Differentiate w.r.t x the following functions:

(a) $\frac{3}{5}x^2 - 2x^7 + \frac{1}{8} - \sqrt{x}$

(b) $(2x^2 - 1)(x^4 - 1)$

(c) $\left(x^5 + \frac{1}{x}\right)(x^5 + 1)$

Q3. Differentiate w.r.t x the following functions:

(a) $\frac{\sqrt{x} - 2}{\sqrt{x} + 1}$

(b) $\frac{x^2 - 1}{x^2 + 1}$

(c) $\frac{x^2 + x + 1}{x^2 - x + 1}$

$$1(a) \ 1 \quad (b) \ 1+2x \quad (c) \ 15x^4 + 8x^3$$

$$(d) \ 32x^3 + 2x^{-\frac{1}{2}} \quad (e) \ \frac{1}{2} - 3x + 15x^2$$

$$(f) -2bc^6$$

$$2(a) \ \frac{6}{5}x - 14x^6 - \frac{1}{2}x^{-\frac{1}{2}}$$

$$(b) \ (4x^3)(x^4-1) + (2x^2-1)(4x^3)$$

$$(c) \ (5x^4 + x^{-2})(x^5+1) + (2x^5 + \frac{1}{x})(5x^4)$$

$$3(a) \ (\frac{1}{2}x^{-\frac{1}{2}})\left(\frac{1}{\sqrt{x}+1}\right) + (\sqrt{x}-2)(\sqrt{x}+1)^{-2}\left(\frac{1}{2}x^{-\frac{1}{2}}\right)$$

$$(b) \ \frac{(2x)(x^2+1) - (x^2-1)(2x)}{(x^2+1)^2}$$

$$(c) \ \frac{(2x+1)(x^2-x+1) - (x^2+x+1)(2x-1)}{(x^2-x+1)^2}$$

2.3 Chain Rule ★ — chpt 6.8

If y is a differentiable function of u , and u is a differentiable function of x , then y is a differentiable function of x , and

$$\frac{dy}{dx} = \frac{dy}{du} \cdot \frac{du}{dx}$$

Questions :

1. Use the chain rule (6.8.1) to find dy/dx for the following:

(a) $y = 5u^4$, where $u = 1 + x^2$

(b) $y = u - u^6$, where $u = 1 + 1/x$

2. Compute the following:

(a) dY/dt , when $Y = -3(V + 1)^5$ and $V = \frac{1}{3}t^3$.

(b) dK/dt , when $K = AL^a$ and $L = bt + c$, where A, a, b , and c are positive constants.

Answer:

$$1(a) \frac{dy}{dx} = 20u^3 (2x)$$

$$= 20(1+x^2)^3(2x)$$

$$(b) \frac{dy}{dx} = (1-6u^5)(-x^{-2})$$

$$= (1-1(1+\frac{1}{x})^5)(-x^{-2})$$

$$2(a) \frac{dy}{dt} = [-15(1+t^3)^4](t^2)$$

$$= [-15(\frac{1}{3}t^3+1)^4](t^2)$$

2.4 Higher Order Derivatives — Chpt 6.09

$$\frac{d^2y}{dx^2} = \frac{d}{dx} \left(\frac{dy}{dx} \right)$$

Question

Compute the second derivatives of:

(a) $y = x^5 - 3x^4 + 2$

(b) $y = (1 + x^2)^{10}$

Ans:

$$(a) \frac{dy}{dx} = 5x^4 - 12x^3$$

$$\frac{d^2y}{dx^2} = 20x^3 - 36x^2$$

$$(b) \frac{dy}{dx} = 10(1+x^2)^9 \cdot 2x$$
$$= 20x (1+x^2)^9$$

$$\frac{d^2y}{dx^2} = 20(1+x^2)^9 + 20x \cdot 9(1+x^2)^8 \cdot 2x$$

2.5 Exponential — Chpt 6.10

$$f(x) = e^x \implies f'(x) = e^x$$

$$f(x) = e^{g(x)} \quad f'(x) = g'(x)e^{g(x)}$$

Questions:

Find the first and second derivatives of:

(a) $y = e^{-3x}$

(b) $y = 2e^{x^3}$

(c) $y = e^{1/x}$

(d) $y = 5e^{2x^2-3x+1}$

Ans:

$$(a) -3e^{-3x}$$

$$(b) 6x^2 e^{x^3}$$

$$(c) -x^2 e^{\frac{1}{x}}$$

$$(d) (4x + 3) \cdot 5e^{2x^2 - 3x + 1}$$

2.6 Logarithmic — Chpt 6.11

$$y = \ln h(x) \Rightarrow y' = \frac{h'(x)}{h(x)}$$

Questions

Find the derivatives of:

(a) $y = x^3(\ln x)^2$

(b) $y = \frac{x^2}{\ln x}$

(c) $y = (\ln x)^{10}$

(d) $y = (\ln x + 3x)^2$

Ans:

$$(a) 3x^2 (\ln x^2) + (3x^2) (2 \ln x) \left(\frac{1}{x}\right)$$

$$(b) \frac{2x \cdot \ln x - \frac{1}{x} \cdot x^2}{(\ln x)^2}$$

$$(c) 10 \cdot (\ln x)^9 \cdot \frac{1}{x}$$

$$(d) 2 (\ln x + 3x) \cdot \left(\frac{1}{x} + 3\right)$$